[WIP] prove everything except the hard bit :)

backend/CMinorEliminateSkip.v
@@ -20,6 +20,10 @@ Require Import Switch Cminor Selectionproof.
 Require Import Errors.
 
 
+Fixpoint measure(st: Cminor.state) : nat :=
+  match st with
+  | _ => 0
+  end.
 
 Fixpoint remove_skip_from_seq_stmt(s: stmt) : stmt :=
   match s with
@@ -85,10 +89,123 @@ Proof.
   rewrite <- H.
   apply match_transform_program; auto.
 Qed.
-  
-Theorem transf_program_correct: forall (p p': Cminor.program),
-    match_prog p p' ->
-    forward_simulation (Cminor.semantics p) (Cminor.semantics p').
+
+Section PRESERVATION.
+  Variable prog tprog: Cminor.program.
+  Hypothesis TRANSL: match_prog prog tprog.
+
+  Let ge := Genv.globalenv prog.
+  Let tge := Genv.globalenv tprog.
+
+  (* TODO: understand what the fuck these are doing *)
+ Lemma symbols_preserved:
+  forall (s: ident), Genv.find_symbol tge s = Genv.find_symbol ge s.
+ Proof.
+   eapply Genv.find_symbol_transf.
+   apply TRANSL.
+ Qed.
+
+Lemma functions_translated:
+  forall (v: val) (f: Cminor.fundef),
+  Genv.find_funct ge v = Some f ->
+  Genv.find_funct tge v = Some (transf_fundef f).
+Proof.
+  apply (Genv.find_funct_transf TRANSL).
+Qed.
+
+Lemma funct_ptr_translated:
+  forall (b: block) (f: Cminor.fundef),
+  Genv.find_funct_ptr ge b = Some f ->
+  Genv.find_funct_ptr tge b = Some (transf_fundef f).
+Proof.
+  apply (Genv.find_funct_ptr_transf TRANSL).
+Qed.
+
+Lemma senv_preserved:
+  Senv.equiv ge tge.
+Proof. apply (Genv.senv_transf TRANSL). Qed.
+
+Lemma sig_preserved:
+  forall f, funsig (transf_fundef f) = funsig f.
+Proof.
+  destruct f; auto. 
+Qed.
+
+Inductive match_states: Cminor.state -> Cminor.state -> Prop :=
+| match_callstates: forall (fdef: fundef)
+                      (args: list val)
+                      (k: cont)
+                      (m: mem),
+    match_states (Callstate fdef args k m)
+                 (Callstate (transf_fundef fdef) args k m)
+| match_state: forall (f: function)  (s: stmt)
+                 (k: cont)
+                 (sp: val)
+                 (e: env)
+                 (m: mem),
+    s <> Sskip -> match_states (State f s k sp e m)
+                             (State (transf_fn f) s k sp e m)
+
+| match_returnstates: forall (v: val)
+                        (k: cont)
+                        (m: mem),
+    match_states (Returnstate v k m) (Returnstate v k m).
+
+Lemma transf_initial_states:
+  forall st1, initial_state prog st1 ->
+  exists st2, initial_state tprog st2 /\ match_states st1 st2.
 Proof.
   intros.
+  inversion H.
+  subst.
+  exists (Callstate (transf_fundef f) nil Kstop m0).
+  split; try constructor.
+  
+  - econstructor; try auto.
+    
+    + apply (Genv.init_mem_transf TRANSL). auto.
+
+    + replace (prog_main tprog) with (prog_main prog).
+      rewrite symbols_preserved. eauto.
+      symmetry;
+      (* comes from Linking *)
+        eapply match_program_main; eauto.
+
+      
+    + subst.
+      
+      assert (Genv.find_funct_ptr tge b = Some (transf_fundef f)).
+      apply funct_ptr_translated.
+      auto.
+      replace (Genv.globalenv tprog) with tge; try auto.
+
+    + rewrite sig_preserved.
+      auto.
+Qed.
+
+Lemma transf_final_states:
+  forall st1 st2 r,
+    match_states  st1 st2 -> final_state st1 r -> final_state st2 r.
+Proof.
+  intros.
+  inversion H0; inversion H; subst; try discriminate.
+
+  rename H0 into FINAL_STATE.
+  rename H3 into STATE_EQ_FINAL_STATE.
+  rewrite <- STATE_EQ_FINAL_STATE in FINAL_STATE.
+  auto.
+Qed.
+
+
+
+Theorem transf_program_correct:
+    forward_simulation (Cminor.semantics prog) (Cminor.semantics tprog).
+Proof.
+  eapply forward_simulation_opt with (match_states := match_states)
+                                     (measure := measure).
+ 
+  - apply senv_preserved.
+  - apply transf_initial_states.
+  - apply transf_final_states.
+  - admit.
 Admitted.
